<?xml version="1.0"?>
<rdf:RDF xmlns="http://www.hsu-hh.de/aut/ontologies/KI1/agents#"
     xml:base="http://www.hsu-hh.de/aut/ontologies/KI1/agents"
     xmlns:owl="http://www.w3.org/2002/07/owl#"
     xmlns:rdf="http://www.w3.org/1999/02/22-rdf-syntax-ns#"
     xmlns:xml="http://www.w3.org/XML/1998/namespace"
     xmlns:xsd="http://www.w3.org/2001/XMLSchema#"
     xmlns:rdfs="http://www.w3.org/2000/01/rdf-schema#"
     xmlns:Agent="http://hsu-hh.de/aut/ontologies/KI1/agents#"
     xmlns:swrla="http://swrl.stanford.edu/ontologies/3.3/swrla.owl#"
     xmlns:agents="http://www.hsu-hh.de/aut/ontologies/KI1/agents#"
     xmlns:VDI3682="http://www.hsu-ifa.de/ontologies/VDI3682#"
     xmlns:DINEN61360="http://www.hsu-ifa.de/ontologies/DINEN61360#"
     xmlns:agent-summer-school="http://www.hsu-hh.de/aut/ontologies/agent-summer-school#">
    <owl:Ontology rdf:about="http://www.hsu-hh.de/aut/ontologies/agent-summer-school">
        <owl:imports rdf:resource="https://raw.githubusercontent.com/hsu-aut/IndustrialStandard-ODP-DINEN61360/v1.4.2/DINEN61360.owl"/>
        <owl:imports rdf:resource="https://raw.githubusercontent.com/hsu-aut/IndustrialStandard-ODP-VDI3682/v3.0.1/VDI3682.owl"/>
        <owl:versionInfo>1.2.0</owl:versionInfo>
        <owl:versionInfo>3.0.1</owl:versionInfo>
    </owl:Ontology>
    


    <!-- 
    ///////////////////////////////////////////////////////////////////////////////////////
    //
    // Annotation properties
    //
    ///////////////////////////////////////////////////////////////////////////////////////
     -->

    


    <!-- http://swrl.stanford.edu/ontologies/3.3/swrla.owl#isRuleEnabled -->

    <owl:AnnotationProperty rdf:about="http://swrl.stanford.edu/ontologies/3.3/swrla.owl#isRuleEnabled"/>
    


    <!-- 
    ///////////////////////////////////////////////////////////////////////////////////////
    //
    // Object Properties
    //
    ///////////////////////////////////////////////////////////////////////////////////////
     -->

    


    <!-- http://www.hsu-hh.de/aut/ontologies/agent-summer-school#hasCapability -->

    <owl:ObjectProperty rdf:about="http://www.hsu-hh.de/aut/ontologies/agent-summer-school#hasCapability">
        <rdfs:domain rdf:resource="http://www.hsu-hh.de/aut/ontologies/agent-summer-school#Agent"/>
        <rdfs:range rdf:resource="http://www.hsu-hh.de/aut/ontologies/agent-summer-school#Capability"/>
    </owl:ObjectProperty>
    


    <!-- http://www.hsu-hh.de/aut/ontologies/agent-summer-school#hasInputProperty -->

    <owl:ObjectProperty rdf:about="http://www.hsu-hh.de/aut/ontologies/agent-summer-school#hasInputProperty">
        <owl:propertyChainAxiom rdf:parseType="Collection">
            <rdf:Description rdf:about="http://www.hsu-ifa.de/ontologies/VDI3682#hasInput"/>
            <rdf:Description rdf:about="http://www.hsu-ifa.de/ontologies/DINEN61360#has_Data_Element"/>
        </owl:propertyChainAxiom>
    </owl:ObjectProperty>
    


    <!-- http://www.hsu-hh.de/aut/ontologies/agent-summer-school#hasInputPropertyType -->

    <owl:ObjectProperty rdf:about="http://www.hsu-hh.de/aut/ontologies/agent-summer-school#hasInputPropertyType">
        <owl:propertyChainAxiom rdf:parseType="Collection">
            <rdf:Description rdf:about="http://www.hsu-hh.de/aut/ontologies/agent-summer-school#hasInputProperty"/>
            <rdf:Description rdf:about="http://www.hsu-ifa.de/ontologies/DINEN61360#has_Type_Description"/>
        </owl:propertyChainAxiom>
    </owl:ObjectProperty>
    


    <!-- http://www.hsu-hh.de/aut/ontologies/agent-summer-school#hasOutputProperty -->

    <owl:ObjectProperty rdf:about="http://www.hsu-hh.de/aut/ontologies/agent-summer-school#hasOutputProperty">
        <owl:propertyChainAxiom rdf:parseType="Collection">
            <rdf:Description rdf:about="http://www.hsu-ifa.de/ontologies/VDI3682#hasOutput"/>
            <rdf:Description rdf:about="http://www.hsu-ifa.de/ontologies/DINEN61360#has_Data_Element"/>
        </owl:propertyChainAxiom>
    </owl:ObjectProperty>
    


    <!-- http://www.hsu-hh.de/aut/ontologies/agent-summer-school#hasOutputPropertyType -->

    <owl:ObjectProperty rdf:about="http://www.hsu-hh.de/aut/ontologies/agent-summer-school#hasOutputPropertyType">
        <owl:propertyChainAxiom rdf:parseType="Collection">
            <rdf:Description rdf:about="http://www.hsu-hh.de/aut/ontologies/agent-summer-school#hasOutputProperty"/>
            <rdf:Description rdf:about="http://www.hsu-ifa.de/ontologies/DINEN61360#has_Type_Description"/>
        </owl:propertyChainAxiom>
    </owl:ObjectProperty>
    


    <!-- http://www.hsu-ifa.de/ontologies/DINEN61360#Data_Element_describes -->

    <owl:ObjectProperty rdf:about="http://www.hsu-ifa.de/ontologies/DINEN61360#Data_Element_describes">
        <owl:inverseOf rdf:resource="http://www.hsu-ifa.de/ontologies/DINEN61360#has_Data_Element"/>
        <rdfs:domain rdf:resource="http://www.hsu-ifa.de/ontologies/DINEN61360#Data_Element"/>
        <rdfs:comment>Description:
This ObjectProperty is used to connect a data element with any kind of entity that is described by the data element</rdfs:comment>
    </owl:ObjectProperty>
    


    <!-- http://www.hsu-ifa.de/ontologies/DINEN61360#Instance_Description_has_Type -->

    <owl:ObjectProperty rdf:about="http://www.hsu-ifa.de/ontologies/DINEN61360#Instance_Description_has_Type">
        <owl:inverseOf rdf:resource="http://www.hsu-ifa.de/ontologies/DINEN61360#Type_Description_has_Instance"/>
        <rdfs:domain rdf:resource="http://www.hsu-ifa.de/ontologies/DINEN61360#Instance_Description"/>
        <rdfs:range rdf:resource="http://www.hsu-ifa.de/ontologies/DINEN61360#Type_Description"/>
    </owl:ObjectProperty>
    


    <!-- http://www.hsu-ifa.de/ontologies/DINEN61360#Type_Description_has_Instance -->

    <owl:ObjectProperty rdf:about="http://www.hsu-ifa.de/ontologies/DINEN61360#Type_Description_has_Instance">
        <rdfs:domain rdf:resource="http://www.hsu-ifa.de/ontologies/DINEN61360#Type_Description"/>
        <rdfs:range rdf:resource="http://www.hsu-ifa.de/ontologies/DINEN61360#Instance_Description"/>
    </owl:ObjectProperty>
    


    <!-- http://www.hsu-ifa.de/ontologies/DINEN61360#complex_Data_Type_has_Member -->

    <owl:ObjectProperty rdf:about="http://www.hsu-ifa.de/ontologies/DINEN61360#complex_Data_Type_has_Member">
        <owl:inverseOf rdf:resource="http://www.hsu-ifa.de/ontologies/DINEN61360#is_Member_of_Complex_Data_Type"/>
        <rdfs:domain>
            <owl:Class>
                <owl:intersectionOf rdf:parseType="Collection">
                    <rdf:Description rdf:about="http://www.hsu-ifa.de/ontologies/DINEN61360#Instance_Description"/>
                    <owl:Restriction>
                        <owl:onProperty rdf:resource="http://www.hsu-ifa.de/ontologies/DINEN61360#Instance_Description_has_Type"/>
                        <owl:allValuesFrom rdf:resource="http://www.hsu-ifa.de/ontologies/DINEN61360#Complex_Data_Type"/>
                    </owl:Restriction>
                </owl:intersectionOf>
            </owl:Class>
        </rdfs:domain>
        <rdfs:range rdf:resource="http://www.hsu-ifa.de/ontologies/DINEN61360#Complex_Data_Type_Member"/>
        <rdfs:comment>Description:
ObjectProperty that is used to connect an instance of a complex data type with corresponding members of the complex data type. These members are connected to types and instances of other (complex) data types</rdfs:comment>
    </owl:ObjectProperty>
    


    <!-- http://www.hsu-ifa.de/ontologies/DINEN61360#has_Data_Element -->

    <owl:ObjectProperty rdf:about="http://www.hsu-ifa.de/ontologies/DINEN61360#has_Data_Element">
        <rdfs:range rdf:resource="http://www.hsu-ifa.de/ontologies/DINEN61360#Data_Element"/>
        <rdfs:comment>Description:
This ObjectProperty is used to connect any kind of entity with a data element that is used for its description.</rdfs:comment>
    </owl:ObjectProperty>
    


    <!-- http://www.hsu-ifa.de/ontologies/DINEN61360#has_Instance_Description -->

    <owl:ObjectProperty rdf:about="http://www.hsu-ifa.de/ontologies/DINEN61360#has_Instance_Description">
        <owl:inverseOf rdf:resource="http://www.hsu-ifa.de/ontologies/DINEN61360#is_Instance_Description_of_Data_Element"/>
        <rdf:type rdf:resource="http://www.w3.org/2002/07/owl#InverseFunctionalProperty"/>
        <rdfs:domain>
            <owl:Class>
                <owl:unionOf rdf:parseType="Collection">
                    <rdf:Description rdf:about="http://www.hsu-ifa.de/ontologies/DINEN61360#Complex_Data_Type_Member"/>
                    <rdf:Description rdf:about="http://www.hsu-ifa.de/ontologies/DINEN61360#Data_Element"/>
                </owl:unionOf>
            </owl:Class>
        </rdfs:domain>
        <rdfs:range rdf:resource="http://www.hsu-ifa.de/ontologies/DINEN61360#Instance_Description"/>
        <rdfs:comment>Description:
ObjectProperty is used to connect an individual that needs to be described by DataProperties with the Instance Description of that properties.</rdfs:comment>
    </owl:ObjectProperty>
    


    <!-- http://www.hsu-ifa.de/ontologies/DINEN61360#has_Type_Description -->

    <owl:ObjectProperty rdf:about="http://www.hsu-ifa.de/ontologies/DINEN61360#has_Type_Description">
        <owl:inverseOf rdf:resource="http://www.hsu-ifa.de/ontologies/DINEN61360#is_Type_Description_of_Data_Element"/>
        <rdf:type rdf:resource="http://www.w3.org/2002/07/owl#FunctionalProperty"/>
        <rdfs:domain>
            <owl:Class>
                <owl:unionOf rdf:parseType="Collection">
                    <rdf:Description rdf:about="http://www.hsu-ifa.de/ontologies/DINEN61360#Complex_Data_Type_Member"/>
                    <rdf:Description rdf:about="http://www.hsu-ifa.de/ontologies/DINEN61360#Data_Element"/>
                </owl:unionOf>
            </owl:Class>
        </rdfs:domain>
        <rdfs:range rdf:resource="http://www.hsu-ifa.de/ontologies/DINEN61360#Type_Description"/>
        <rdfs:comment>Description:
ObjectProperty is used to connect an individual that needs to be described by DataProperties with the Type Description of that properties.

Functional:
Any indivudual representing a property, can have only one Type Description</rdfs:comment>
    </owl:ObjectProperty>
    


    <!-- http://www.hsu-ifa.de/ontologies/DINEN61360#is_Instance_Description_of_Data_Element -->

    <owl:ObjectProperty rdf:about="http://www.hsu-ifa.de/ontologies/DINEN61360#is_Instance_Description_of_Data_Element">
        <rdfs:comment>Description:
ObjectProperty is used to connect an Instance Description with the Data_Element that it describes.

Inverse of has_Instance_Description</rdfs:comment>
    </owl:ObjectProperty>
    


    <!-- http://www.hsu-ifa.de/ontologies/DINEN61360#is_Member_of_Complex_Data_Type -->

    <owl:ObjectProperty rdf:about="http://www.hsu-ifa.de/ontologies/DINEN61360#is_Member_of_Complex_Data_Type">
        <rdfs:domain rdf:resource="http://www.hsu-ifa.de/ontologies/DINEN61360#Complex_Data_Type_Member"/>
        <rdfs:range>
            <owl:Class>
                <owl:intersectionOf rdf:parseType="Collection">
                    <rdf:Description rdf:about="http://www.hsu-ifa.de/ontologies/DINEN61360#Instance_Description"/>
                    <owl:Restriction>
                        <owl:onProperty rdf:resource="http://www.hsu-ifa.de/ontologies/DINEN61360#Instance_Description_has_Type"/>
                        <owl:allValuesFrom rdf:resource="http://www.hsu-ifa.de/ontologies/DINEN61360#Complex_Data_Type"/>
                    </owl:Restriction>
                </owl:intersectionOf>
            </owl:Class>
        </rdfs:range>
    </owl:ObjectProperty>
    


    <!-- http://www.hsu-ifa.de/ontologies/DINEN61360#is_Type_Description_of_Data_Element -->

    <owl:ObjectProperty rdf:about="http://www.hsu-ifa.de/ontologies/DINEN61360#is_Type_Description_of_Data_Element">
        <rdfs:comment>Description:
ObjectProperty is used to connect a Type_Description with a Data_Element that has instace descriptions of this type. 

Inverse of has_Type_Description</rdfs:comment>
    </owl:ObjectProperty>
    


    <!-- http://www.hsu-ifa.de/ontologies/VDI3682#consistsOf -->

    <owl:ObjectProperty rdf:about="http://www.hsu-ifa.de/ontologies/VDI3682#consistsOf">
        <rdfs:subPropertyOf rdf:resource="http://www.w3.org/2002/07/owl#topObjectProperty"/>
        <rdfs:domain rdf:resource="http://www.hsu-ifa.de/ontologies/VDI3682#Process"/>
        <rdfs:range>
            <owl:Class>
                <owl:unionOf rdf:parseType="Collection">
                    <rdf:Description rdf:about="http://www.hsu-ifa.de/ontologies/VDI3682#ProcessOperator"/>
                    <rdf:Description rdf:about="http://www.hsu-ifa.de/ontologies/VDI3682#State"/>
                    <rdf:Description rdf:about="http://www.hsu-ifa.de/ontologies/VDI3682#SystemLimit"/>
                </owl:unionOf>
            </owl:Class>
        </rdfs:range>
        <rdfs:comment xml:lang="en">Describes containment of process elements (state, process operator, system limit) within a process</rdfs:comment>
    </owl:ObjectProperty>
    


    <!-- http://www.hsu-ifa.de/ontologies/VDI3682#dependency -->

    <owl:ObjectProperty rdf:about="http://www.hsu-ifa.de/ontologies/VDI3682#dependency">
        <rdfs:domain rdf:resource="http://www.hsu-ifa.de/ontologies/VDI3682#State"/>
        <rdfs:range rdf:resource="http://www.hsu-ifa.de/ontologies/VDI3682#State"/>
        <rdfs:comment xml:lang="en">This ObjectProperty is not explicitly contained within the VDI 3682. It is used to describe dependencies of In- and Outputs. Due to open world assumption (OWA) the case that more than one In- or Outputs occur does always mean an alternative Input. For the case, that In- and Outputs are depending on each other, the ObjectProperty Dependency can be used. It can be interpreted as an &quot;AND&quot; constructor between In- and/or Outputs of a process.

E.g.: A process has two Inputs. If they are alternatives, then this fact must not  be explcitly modelled. If both Inputs have to go into the process, then the &quot;Dependency&quot; ObjectProperty is assigned between them.

More complex example: Input A and B have to go into a process, while Input C and D are alternatives for A and B. The Inputs have to go as groups in the process. This equals: A AND B OR C AND D. The Dependency Operator is used between A and B as well as between C and D.

Furthermore, the Operator can be used to express dependencies between In- and Outputs. If A and B are alternative Inputs that result in the Ouputs C for A or D for B then this equals: A AND C or D AND B. The ObjectProperty can be used between both, In- and/or Outputs.</rdfs:comment>
    </owl:ObjectProperty>
    


    <!-- http://www.hsu-ifa.de/ontologies/VDI3682#flow -->

    <owl:ObjectProperty rdf:about="http://www.hsu-ifa.de/ontologies/VDI3682#flow">
        <rdfs:comment>most generic concept for flows taken from VDI3682 and refined by semantics that is used in graphical notation</rdfs:comment>
    </owl:ObjectProperty>
    


    <!-- http://www.hsu-ifa.de/ontologies/VDI3682#hasAlternativeInput -->

    <owl:ObjectProperty rdf:about="http://www.hsu-ifa.de/ontologies/VDI3682#hasAlternativeInput">
        <rdfs:subPropertyOf rdf:resource="http://www.hsu-ifa.de/ontologies/VDI3682#hasInput"/>
    </owl:ObjectProperty>
    


    <!-- http://www.hsu-ifa.de/ontologies/VDI3682#hasAlternativeOutput -->

    <owl:ObjectProperty rdf:about="http://www.hsu-ifa.de/ontologies/VDI3682#hasAlternativeOutput">
        <rdfs:subPropertyOf rdf:resource="http://www.hsu-ifa.de/ontologies/VDI3682#hasOutput"/>
    </owl:ObjectProperty>
    


    <!-- http://www.hsu-ifa.de/ontologies/VDI3682#hasInput -->

    <owl:ObjectProperty rdf:about="http://www.hsu-ifa.de/ontologies/VDI3682#hasInput">
        <rdfs:subPropertyOf rdf:resource="http://www.hsu-ifa.de/ontologies/VDI3682#flow"/>
        <rdfs:domain>
            <owl:Class>
                <owl:unionOf rdf:parseType="Collection">
                    <rdf:Description rdf:about="http://www.hsu-ifa.de/ontologies/VDI3682#Process"/>
                    <rdf:Description rdf:about="http://www.hsu-ifa.de/ontologies/VDI3682#ProcessOperator"/>
                </owl:unionOf>
            </owl:Class>
        </rdfs:domain>
        <rdfs:range rdf:resource="http://www.hsu-ifa.de/ontologies/VDI3682#State"/>
        <rdfs:comment>ObjectProperty that is used to link a ProcessOperator with an Input, i.e. Energy or Information or Product.</rdfs:comment>
    </owl:ObjectProperty>
    


    <!-- http://www.hsu-ifa.de/ontologies/VDI3682#hasOutput -->

    <owl:ObjectProperty rdf:about="http://www.hsu-ifa.de/ontologies/VDI3682#hasOutput">
        <rdfs:subPropertyOf rdf:resource="http://www.hsu-ifa.de/ontologies/VDI3682#flow"/>
        <rdfs:domain>
            <owl:Class>
                <owl:unionOf rdf:parseType="Collection">
                    <rdf:Description rdf:about="http://www.hsu-ifa.de/ontologies/VDI3682#Process"/>
                    <rdf:Description rdf:about="http://www.hsu-ifa.de/ontologies/VDI3682#ProcessOperator"/>
                </owl:unionOf>
            </owl:Class>
        </rdfs:domain>
        <rdfs:range rdf:resource="http://www.hsu-ifa.de/ontologies/VDI3682#State"/>
        <rdfs:comment>ObjectProperty that is used to link a ProcessOperator with an Output, i.e. Energy or Information or Product.</rdfs:comment>
    </owl:ObjectProperty>
    


    <!-- http://www.hsu-ifa.de/ontologies/VDI3682#hasParallelInput -->

    <owl:ObjectProperty rdf:about="http://www.hsu-ifa.de/ontologies/VDI3682#hasParallelInput">
        <rdfs:subPropertyOf rdf:resource="http://www.hsu-ifa.de/ontologies/VDI3682#hasInput"/>
    </owl:ObjectProperty>
    


    <!-- http://www.hsu-ifa.de/ontologies/VDI3682#hasParallelOutput -->

    <owl:ObjectProperty rdf:about="http://www.hsu-ifa.de/ontologies/VDI3682#hasParallelOutput">
        <rdfs:subPropertyOf rdf:resource="http://www.hsu-ifa.de/ontologies/VDI3682#hasOutput"/>
    </owl:ObjectProperty>
    


    <!-- http://www.hsu-ifa.de/ontologies/VDI3682#hasPredecessor -->

    <owl:ObjectProperty rdf:about="http://www.hsu-ifa.de/ontologies/VDI3682#hasPredecessor">
        <owl:inverseOf rdf:resource="http://www.hsu-ifa.de/ontologies/VDI3682#hasSuccessor"/>
        <rdf:type rdf:resource="http://www.w3.org/2002/07/owl#TransitiveProperty"/>
        <rdfs:domain rdf:resource="http://www.hsu-ifa.de/ontologies/VDI3682#ProcessOperator"/>
        <rdfs:range rdf:resource="http://www.hsu-ifa.de/ontologies/VDI3682#ProcessOperator"/>
        <owl:propertyChainAxiom rdf:parseType="Collection">
            <rdf:Description rdf:about="http://www.hsu-ifa.de/ontologies/VDI3682#hasInput"/>
            <rdf:Description>
                <owl:inverseOf rdf:resource="http://www.hsu-ifa.de/ontologies/VDI3682#hasOutput"/>
            </rdf:Description>
        </owl:propertyChainAxiom>
        <rdfs:comment>an object property that is used to infer a predecessing relationship between entities</rdfs:comment>
    </owl:ObjectProperty>
    


    <!-- http://www.hsu-ifa.de/ontologies/VDI3682#hasSubProcess -->

    <owl:ObjectProperty rdf:about="http://www.hsu-ifa.de/ontologies/VDI3682#hasSubProcess">
        <rdf:type rdf:resource="http://www.w3.org/2002/07/owl#TransitiveProperty"/>
        <rdfs:domain>
            <owl:Class>
                <owl:unionOf rdf:parseType="Collection">
                    <rdf:Description rdf:about="http://www.hsu-ifa.de/ontologies/VDI3682#Process"/>
                    <rdf:Description rdf:about="http://www.hsu-ifa.de/ontologies/VDI3682#ProcessOperator"/>
                </owl:unionOf>
            </owl:Class>
        </rdfs:domain>
        <rdfs:range rdf:resource="http://www.hsu-ifa.de/ontologies/VDI3682#Process"/>
        <owl:propertyChainAxiom rdf:parseType="Collection">
            <rdf:Description rdf:about="http://www.hsu-ifa.de/ontologies/VDI3682#isComposedOf"/>
            <rdf:Description>
                <owl:inverseOf rdf:resource="http://www.hsu-ifa.de/ontologies/VDI3682#consistsOf"/>
            </rdf:Description>
        </owl:propertyChainAxiom>
        <rdfs:comment>Is used to find the complete decomposed process of a process operatore. Note: This is syntactic sugar as a subprocess can be found by following &quot;isComposedOf&quot; and the inverse of &quot;consistsOf&quot;.</rdfs:comment>
    </owl:ObjectProperty>
    


    <!-- http://www.hsu-ifa.de/ontologies/VDI3682#hasSuccessor -->

    <owl:ObjectProperty rdf:about="http://www.hsu-ifa.de/ontologies/VDI3682#hasSuccessor">
        <rdf:type rdf:resource="http://www.w3.org/2002/07/owl#TransitiveProperty"/>
        <rdfs:domain rdf:resource="http://www.hsu-ifa.de/ontologies/VDI3682#ProcessOperator"/>
        <rdfs:range rdf:resource="http://www.hsu-ifa.de/ontologies/VDI3682#ProcessOperator"/>
        <owl:propertyChainAxiom rdf:parseType="Collection">
            <rdf:Description rdf:about="http://www.hsu-ifa.de/ontologies/VDI3682#hasOutput"/>
            <rdf:Description>
                <owl:inverseOf rdf:resource="http://www.hsu-ifa.de/ontologies/VDI3682#hasInput"/>
            </rdf:Description>
        </owl:propertyChainAxiom>
        <rdfs:comment>an object property that is used to infer a successing relationshipt between entities</rdfs:comment>
    </owl:ObjectProperty>
    


    <!-- http://www.hsu-ifa.de/ontologies/VDI3682#hasUpperProcess -->

    <owl:ObjectProperty rdf:about="http://www.hsu-ifa.de/ontologies/VDI3682#hasUpperProcess">
        <rdfs:domain>
            <owl:Class>
                <owl:unionOf rdf:parseType="Collection">
                    <rdf:Description rdf:about="http://www.hsu-ifa.de/ontologies/VDI3682#Process"/>
                    <rdf:Description rdf:about="http://www.hsu-ifa.de/ontologies/VDI3682#ProcessOperator"/>
                </owl:unionOf>
            </owl:Class>
        </rdfs:domain>
        <rdfs:range rdf:resource="http://www.hsu-ifa.de/ontologies/VDI3682#Process"/>
        <owl:propertyChainAxiom rdf:parseType="Collection">
            <rdf:Description>
                <owl:inverseOf rdf:resource="http://www.hsu-ifa.de/ontologies/VDI3682#isComposedOf"/>
            </rdf:Description>
            <rdf:Description>
                <owl:inverseOf rdf:resource="http://www.hsu-ifa.de/ontologies/VDI3682#consistsOf"/>
            </rdf:Description>
        </owl:propertyChainAxiom>
        <rdfs:comment>Is used to find the parent (upper) process of a lower level process operator. Note: This is syntactic sugar as a parent process can be found by following the inverse of &quot;isComposedOf&quot; and the inverse of &quot;consistsOf&quot;.</rdfs:comment>
    </owl:ObjectProperty>
    


    <!-- http://www.hsu-ifa.de/ontologies/VDI3682#isAssignedTo -->

    <owl:ObjectProperty rdf:about="http://www.hsu-ifa.de/ontologies/VDI3682#isAssignedTo">
        <rdfs:domain rdf:resource="http://www.hsu-ifa.de/ontologies/VDI3682#ProcessOperator"/>
        <rdfs:range rdf:resource="http://www.hsu-ifa.de/ontologies/VDI3682#TechnicalResource"/>
        <rdfs:comment>ObjectProperty that is used to indicate that a process operator is performed by a technical resource.</rdfs:comment>
    </owl:ObjectProperty>
    


    <!-- http://www.hsu-ifa.de/ontologies/VDI3682#isComposedOf -->

    <owl:ObjectProperty rdf:about="http://www.hsu-ifa.de/ontologies/VDI3682#isComposedOf">
        <rdfs:domain rdf:resource="http://www.hsu-ifa.de/ontologies/VDI3682#ProcessOperator"/>
        <rdfs:range rdf:resource="http://www.hsu-ifa.de/ontologies/VDI3682#ProcessOperator"/>
        <rdfs:comment>Used for decomposition. A process operator can be composed of multiple more detailed process operators.</rdfs:comment>
    </owl:ObjectProperty>
    


    <!-- 
    ///////////////////////////////////////////////////////////////////////////////////////
    //
    // Data properties
    //
    ///////////////////////////////////////////////////////////////////////////////////////
     -->

    


    <!-- http://www.hsu-hh.de/aut/ontologies/agent-summer-school#allowsMaximumLength -->

    <owl:DatatypeProperty rdf:about="http://www.hsu-hh.de/aut/ontologies/agent-summer-school#allowsMaximumLength"/>
    


    <!-- http://www.hsu-hh.de/aut/ontologies/agent-summer-school#hasLength -->

    <owl:DatatypeProperty rdf:about="http://www.hsu-hh.de/aut/ontologies/agent-summer-school#hasLength">
        <rdfs:domain rdf:resource="http://www.hsu-hh.de/aut/ontologies/agent-summer-school#Product"/>
        <rdfs:range rdf:resource="http://www.w3.org/2001/XMLSchema#decimal"/>
    </owl:DatatypeProperty>
    


    <!-- http://www.hsu-hh.de/aut/ontologies/agent-summer-school#hasPriorityNumber -->

    <owl:DatatypeProperty rdf:about="http://www.hsu-hh.de/aut/ontologies/agent-summer-school#hasPriorityNumber">
        <rdfs:domain rdf:resource="http://www.hsu-hh.de/aut/ontologies/agent-summer-school#Capability"/>
        <rdfs:range rdf:resource="http://www.w3.org/2001/XMLSchema#short"/>
    </owl:DatatypeProperty>
    


    <!-- http://www.hsu-hh.de/aut/ontologies/agent-summer-school#hasProductId -->

    <owl:DatatypeProperty rdf:about="http://www.hsu-hh.de/aut/ontologies/agent-summer-school#hasProductId">
        <rdfs:domain rdf:resource="http://www.hsu-hh.de/aut/ontologies/agent-summer-school#Product"/>
    </owl:DatatypeProperty>
    


    <!-- http://www.hsu-hh.de/aut/ontologies/agent-summer-school#hasUrl -->

    <owl:DatatypeProperty rdf:about="http://www.hsu-hh.de/aut/ontologies/agent-summer-school#hasUrl">
        <rdfs:domain rdf:resource="http://www.hsu-hh.de/aut/ontologies/agent-summer-school#Capability"/>
        <rdfs:range rdf:resource="http://www.w3.org/2001/XMLSchema#string"/>
    </owl:DatatypeProperty>
    


    <!-- http://www.hsu-ifa.de/ontologies/DINEN61360#Array_Member_Dimension -->

    <owl:DatatypeProperty rdf:about="http://www.hsu-ifa.de/ontologies/DINEN61360#Array_Member_Dimension">
        <rdfs:domain rdf:resource="http://www.hsu-ifa.de/ontologies/DINEN61360#Array_Member"/>
        <rdfs:range rdf:resource="http://www.w3.org/2001/XMLSchema#int"/>
        <rdfs:comment>Description:

Indicates the dimension of an array member.</rdfs:comment>
    </owl:DatatypeProperty>
    


    <!-- http://www.hsu-ifa.de/ontologies/DINEN61360#Array_Member_Position -->

    <owl:DatatypeProperty rdf:about="http://www.hsu-ifa.de/ontologies/DINEN61360#Array_Member_Position">
        <rdfs:comment>Description:

DataProperty that indicates the position of an Array_Member in a DataType List.</rdfs:comment>
    </owl:DatatypeProperty>
    


    <!-- http://www.hsu-ifa.de/ontologies/DINEN61360#Boolean_Operator -->

    <owl:DatatypeProperty rdf:about="http://www.hsu-ifa.de/ontologies/DINEN61360#Boolean_Operator">
        <rdf:type rdf:resource="http://www.w3.org/2002/07/owl#FunctionalProperty"/>
        <rdfs:range>
            <rdfs:Datatype>
                <owl:oneOf>
                    <rdf:Description>
                        <rdf:type rdf:resource="http://www.w3.org/1999/02/22-rdf-syntax-ns#List"/>
                        <rdf:first>AND</rdf:first>
                        <rdf:rest>
                            <rdf:Description>
                                <rdf:type rdf:resource="http://www.w3.org/1999/02/22-rdf-syntax-ns#List"/>
                                <rdf:first>NAND</rdf:first>
                                <rdf:rest>
                                    <rdf:Description>
                                        <rdf:type rdf:resource="http://www.w3.org/1999/02/22-rdf-syntax-ns#List"/>
                                        <rdf:first>NOR</rdf:first>
                                        <rdf:rest>
                                            <rdf:Description>
                                                <rdf:type rdf:resource="http://www.w3.org/1999/02/22-rdf-syntax-ns#List"/>
                                                <rdf:first>OR</rdf:first>
                                                <rdf:rest>
                                                    <rdf:Description>
                                                        <rdf:type rdf:resource="http://www.w3.org/1999/02/22-rdf-syntax-ns#List"/>
                                                        <rdf:first>XOR</rdf:first>
                                                        <rdf:rest rdf:resource="http://www.w3.org/1999/02/22-rdf-syntax-ns#nil"/>
                                                    </rdf:Description>
                                                </rdf:rest>
                                            </rdf:Description>
                                        </rdf:rest>
                                    </rdf:Description>
                                </rdf:rest>
                            </rdf:Description>
                        </rdf:rest>
                    </rdf:Description>
                </owl:oneOf>
            </rdfs:Datatype>
        </rdfs:range>
        <rdfs:comment>Is used with Boolean_Association to define what kind of boolean relation connects the Data_Elements of the Boolean_Association</rdfs:comment>
    </owl:DatatypeProperty>
    


    <!-- http://www.hsu-ifa.de/ontologies/DINEN61360#Code -->

    <owl:DatatypeProperty rdf:about="http://www.hsu-ifa.de/ontologies/DINEN61360#Code">
        <rdfs:subPropertyOf rdf:resource="http://www.w3.org/2002/07/owl#topDataProperty"/>
        <rdf:type rdf:resource="http://www.w3.org/2002/07/owl#FunctionalProperty"/>
        <rdfs:domain rdf:resource="http://www.hsu-ifa.de/ontologies/DINEN61360#Type_Description"/>
        <rdfs:comment>Description:
DIN EN 61360-1:2018 Section 7.3
Unique identifier of this data element type. Preferable this should be a standardized identifier (e.g. from eclss or common data dictionary).  optional exlusion of &quot;o&quot; and &quot;i&quot; is not implemented.    

Liability: necessary    

type: string with 6 digits between, first three digits are a-z and last three digits are 0-9  poposed data range expression: xsd:string[pattern &quot;[a-z0-9] {6}&quot;]</rdfs:comment>
    </owl:DatatypeProperty>
    


    <!-- http://www.hsu-ifa.de/ontologies/DINEN61360#Created_at_Date -->

    <owl:DatatypeProperty rdf:about="http://www.hsu-ifa.de/ontologies/DINEN61360#Created_at_Date">
        <rdfs:domain rdf:resource="http://www.hsu-ifa.de/ontologies/DINEN61360#Instance_Description"/>
        <rdfs:range rdf:resource="http://www.w3.org/2001/XMLSchema#dateTimeStamp"/>
        <rdfs:comment>Description: 
A SemAnz40 attribute, that indicates the creation date for an instance.</rdfs:comment>
    </owl:DatatypeProperty>
    


    <!-- http://www.hsu-ifa.de/ontologies/DINEN61360#Definition -->

    <owl:DatatypeProperty rdf:about="http://www.hsu-ifa.de/ontologies/DINEN61360#Definition">
        <rdfs:subPropertyOf rdf:resource="http://www.w3.org/2002/07/owl#topDataProperty"/>
        <rdfs:domain rdf:resource="http://www.hsu-ifa.de/ontologies/DINEN61360#Type_Description"/>
        <rdfs:comment>Description:
A textual definition of the data element

Liability: Necessary

DIN EN 61360-1:2018 Section 8.3

Type: String

Poposed Data Range Expression: xsd:string</rdfs:comment>
    </owl:DatatypeProperty>
    


    <!-- http://www.hsu-ifa.de/ontologies/DINEN61360#Drawing_Reference -->

    <owl:DatatypeProperty rdf:about="http://www.hsu-ifa.de/ontologies/DINEN61360#Drawing_Reference">
        <rdfs:subPropertyOf rdf:resource="http://www.w3.org/2002/07/owl#topDataProperty"/>
        <rdfs:domain rdf:resource="http://www.hsu-ifa.de/ontologies/DINEN61360#Type_Description"/>
        <rdfs:comment>Description:
A link to a drawing (or picture) that is used for further explanation of the data element

Liability: Optional

DIN EN 61360-1:2018 Section 6.13

Type: Contains a URL link as a string to a picture

Poposed Data Range Expression: xsd:string</rdfs:comment>
    </owl:DatatypeProperty>
    


    <!-- http://www.hsu-ifa.de/ontologies/DINEN61360#Expression_Goal -->

    <owl:DatatypeProperty rdf:about="http://www.hsu-ifa.de/ontologies/DINEN61360#Expression_Goal">
        <rdfs:subPropertyOf rdf:resource="http://www.w3.org/2002/07/owl#topDataProperty"/>
        <rdf:type rdf:resource="http://www.w3.org/2002/07/owl#FunctionalProperty"/>
        <rdfs:domain rdf:resource="http://www.hsu-ifa.de/ontologies/DINEN61360#Instance_Description"/>
        <rdfs:range>
            <rdfs:Datatype>
                <owl:oneOf>
                    <rdf:Description>
                        <rdf:type rdf:resource="http://www.w3.org/1999/02/22-rdf-syntax-ns#List"/>
                        <rdf:first>Actual_Value</rdf:first>
                        <rdf:rest>
                            <rdf:Description>
                                <rdf:type rdf:resource="http://www.w3.org/1999/02/22-rdf-syntax-ns#List"/>
                                <rdf:first>Assurance</rdf:first>
                                <rdf:rest>
                                    <rdf:Description>
                                        <rdf:type rdf:resource="http://www.w3.org/1999/02/22-rdf-syntax-ns#List"/>
                                        <rdf:first>Requirement</rdf:first>
                                        <rdf:rest rdf:resource="http://www.w3.org/1999/02/22-rdf-syntax-ns#nil"/>
                                    </rdf:Description>
                                </rdf:rest>
                            </rdf:Description>
                        </rdf:rest>
                    </rdf:Description>
                </owl:oneOf>
            </rdfs:Datatype>
        </rdfs:range>
        <rdfs:comment>Description:

The goal of the values expression, which can be a Requirement, an Assurance or an actual (e.g. measured) value.

Liability: Necessary</rdfs:comment>
    </owl:DatatypeProperty>
    


    <!-- http://www.hsu-ifa.de/ontologies/DINEN61360#Format_DIN61360_SemAnz40 -->

    <owl:DatatypeProperty rdf:about="http://www.hsu-ifa.de/ontologies/DINEN61360#Format_DIN61360_SemAnz40">
        <rdfs:subPropertyOf rdf:resource="http://www.w3.org/2002/07/owl#topDataProperty"/>
        <rdfs:domain rdf:resource="http://www.hsu-ifa.de/ontologies/DINEN61360#Data_Element"/>
        <rdfs:comment>Description: 

Indicates, whether the described type or entity is described by the DIN61360&amp;SemAnz40 Format.

Liability: Necessary

Type: If true, the Data Element is based on the Din61360 and SemAnz40 description

Poposed Data Range Expression: xsd:boolean</rdfs:comment>
    </owl:DatatypeProperty>
    


    <!-- http://www.hsu-ifa.de/ontologies/DINEN61360#Formula -->

    <owl:DatatypeProperty rdf:about="http://www.hsu-ifa.de/ontologies/DINEN61360#Formula">
        <rdfs:subPropertyOf rdf:resource="http://www.w3.org/2002/07/owl#topDataProperty"/>
        <rdfs:domain rdf:resource="http://www.hsu-ifa.de/ontologies/DINEN61360#Type_Description"/>
        <rdfs:comment>Description:
A mathematical euqation that is being used for characterization of the data element

Liability: Optional

DIN EN 61360-1:2018 Section 6.5

Type: contains a URL link as a string to a source file that describes the formula

Poposed Data Range Expression: xsd:string</rdfs:comment>
    </owl:DatatypeProperty>
    


    <!-- http://www.hsu-ifa.de/ontologies/DINEN61360#List_Member_Position -->

    <owl:DatatypeProperty rdf:about="http://www.hsu-ifa.de/ontologies/DINEN61360#List_Member_Position">
        <rdfs:domain rdf:resource="http://www.hsu-ifa.de/ontologies/DINEN61360#List_Member"/>
        <rdfs:range rdf:resource="http://www.w3.org/2001/XMLSchema#int"/>
        <rdfs:comment>Description:

DataProperty that indicates the position of a List_Member in a DataType List.</rdfs:comment>
    </owl:DatatypeProperty>
    


    <!-- http://www.hsu-ifa.de/ontologies/DINEN61360#Logic_Interpretation -->

    <owl:DatatypeProperty rdf:about="http://www.hsu-ifa.de/ontologies/DINEN61360#Logic_Interpretation">
        <rdfs:subPropertyOf rdf:resource="http://www.w3.org/2002/07/owl#topDataProperty"/>
        <rdf:type rdf:resource="http://www.w3.org/2002/07/owl#FunctionalProperty"/>
        <rdfs:domain rdf:resource="http://www.hsu-ifa.de/ontologies/DINEN61360#Instance_Description"/>
        <rdfs:range>
            <rdfs:Datatype>
                <owl:oneOf>
                    <rdf:Description>
                        <rdf:type rdf:resource="http://www.w3.org/1999/02/22-rdf-syntax-ns#List"/>
                        <rdf:first>&lt;</rdf:first>
                        <rdf:rest>
                            <rdf:Description>
                                <rdf:type rdf:resource="http://www.w3.org/1999/02/22-rdf-syntax-ns#List"/>
                                <rdf:first>&lt;=</rdf:first>
                                <rdf:rest>
                                    <rdf:Description>
                                        <rdf:type rdf:resource="http://www.w3.org/1999/02/22-rdf-syntax-ns#List"/>
                                        <rdf:first>=</rdf:first>
                                        <rdf:rest>
                                            <rdf:Description>
                                                <rdf:type rdf:resource="http://www.w3.org/1999/02/22-rdf-syntax-ns#List"/>
                                                <rdf:first>&gt;</rdf:first>
                                                <rdf:rest>
                                                    <rdf:Description>
                                                        <rdf:type rdf:resource="http://www.w3.org/1999/02/22-rdf-syntax-ns#List"/>
                                                        <rdf:first>&gt;=</rdf:first>
                                                        <rdf:rest rdf:resource="http://www.w3.org/1999/02/22-rdf-syntax-ns#nil"/>
                                                    </rdf:Description>
                                                </rdf:rest>
                                            </rdf:Description>
                                        </rdf:rest>
                                    </rdf:Description>
                                </rdf:rest>
                            </rdf:Description>
                        </rdf:rest>
                    </rdf:Description>
                </owl:oneOf>
            </rdfs:Datatype>
        </rdfs:range>
        <rdfs:comment>Description:

Indicates, whether a value with a certain Expression Goal has to be considered as equal (&quot;=&quot;), greater than (&quot;&lt;&quot;), lower than (&quot;&gt;&quot;) or in combination with an equals (i.e. &quot;&lt;=&quot;, &quot;&gt;=&quot;).

Liability: Necessary</rdfs:comment>
    </owl:DatatypeProperty>
    


    <!-- http://www.hsu-ifa.de/ontologies/DINEN61360#Note -->

    <owl:DatatypeProperty rdf:about="http://www.hsu-ifa.de/ontologies/DINEN61360#Note">
        <rdfs:subPropertyOf rdf:resource="http://www.w3.org/2002/07/owl#topDataProperty"/>
        <rdfs:domain rdf:resource="http://www.hsu-ifa.de/ontologies/DINEN61360#Type_Description"/>
        <rdfs:comment>Description:
Additional information that are important to understand the meaning of the data element

Liability: Optional

DIN EN 61360-1:2018 Section 8.4

Type: String

Poposed Data Range Expression: xsd:string</rdfs:comment>
    </owl:DatatypeProperty>
    


    <!-- http://www.hsu-ifa.de/ontologies/DINEN61360#Preferred_Letter_Symbol -->

    <owl:DatatypeProperty rdf:about="http://www.hsu-ifa.de/ontologies/DINEN61360#Preferred_Letter_Symbol">
        <rdfs:subPropertyOf rdf:resource="http://www.w3.org/2002/07/owl#topDataProperty"/>
        <rdfs:domain rdf:resource="http://www.hsu-ifa.de/ontologies/DINEN61360#Type_Description"/>
        <rdfs:comment>Description:
A sign or literal that is used to represent the property (e.g. greek &quot;sigma&quot; for tension))

Liability: Optional

DIN EN 61360-1:2018 Section 6.6

Type: IEC 60027, IEC 60747 or IEC 60148 compliant formula sign described as a string

Poposed Data Range Expression: xsd:string</rdfs:comment>
    </owl:DatatypeProperty>
    


    <!-- http://www.hsu-ifa.de/ontologies/DINEN61360#Preferred_Name -->

    <owl:DatatypeProperty rdf:about="http://www.hsu-ifa.de/ontologies/DINEN61360#Preferred_Name">
        <rdfs:subPropertyOf rdf:resource="http://www.w3.org/2002/07/owl#topDataProperty"/>
        <rdfs:domain rdf:resource="http://www.hsu-ifa.de/ontologies/DINEN61360#Type_Description"/>
        <rdfs:comment>Description:
Represents the preferred name of the data element type, that is being used for searches for instance.

Liability: Necessary

DIN EN 61360-1:2018 Section 7.4

Type: String with lower and upper case, with a maximum of 70 characters

Poposed Data Range Expression: xsd:string[maxLength 70]</rdfs:comment>
    </owl:DatatypeProperty>
    


    <!-- http://www.hsu-ifa.de/ontologies/DINEN61360#Quality -->

    <owl:DatatypeProperty rdf:about="http://www.hsu-ifa.de/ontologies/DINEN61360#Quality">
        <rdfs:subPropertyOf rdf:resource="http://www.w3.org/2002/07/owl#topDataProperty"/>
        <rdfs:domain rdf:resource="http://www.hsu-ifa.de/ontologies/DINEN61360#Instance_Description"/>
        <rdfs:comment>Description:

Not supported so far, since it requires a additional quality ontology</rdfs:comment>
    </owl:DatatypeProperty>
    


    <!-- http://www.hsu-ifa.de/ontologies/DINEN61360#Remark -->

    <owl:DatatypeProperty rdf:about="http://www.hsu-ifa.de/ontologies/DINEN61360#Remark">
        <rdfs:domain rdf:resource="http://www.hsu-ifa.de/ontologies/DINEN61360#Type_Description"/>
        <rdfs:comment>Additional information that can be used to express a oppinion but should not change the meaning of the definition.
DIN EN 61360-1:2018 Section 8.5</rdfs:comment>
    </owl:DatatypeProperty>
    


    <!-- http://www.hsu-ifa.de/ontologies/DINEN61360#Revision_Number -->

    <owl:DatatypeProperty rdf:about="http://www.hsu-ifa.de/ontologies/DINEN61360#Revision_Number">
        <rdfs:subPropertyOf rdf:resource="http://www.w3.org/2002/07/owl#topDataProperty"/>
        <rdfs:domain rdf:resource="http://www.hsu-ifa.de/ontologies/DINEN61360#Type_Description"/>
        <rdfs:comment>Description:
Number that represents the actual count of changes

Liability: Necessary

DIN EN 61360-1:2018 Section 7.5

Type: Integer with two digits between 1 and 99

Poposed Data Range Expression: xsd:integer[&gt;= 1 , &lt;= 99]</rdfs:comment>
    </owl:DatatypeProperty>
    


    <!-- http://www.hsu-ifa.de/ontologies/DINEN61360#Short_Name -->

    <owl:DatatypeProperty rdf:about="http://www.hsu-ifa.de/ontologies/DINEN61360#Short_Name">
        <rdfs:subPropertyOf rdf:resource="http://www.w3.org/2002/07/owl#topDataProperty"/>
        <rdfs:domain rdf:resource="http://www.hsu-ifa.de/ontologies/DINEN61360#Type_Description"/>
        <rdfs:comment>Description:
A short name or acronym that is used for the preferred name

Liability: Necessary

DIN EN 61360-1:2018 Section 7.6

Type: Strong restrictions of DIN61360  not implemented, just strings necessary. Maximum characters is 17.

Poposed Data Range Expression: xsd:string[maxLength 17]</rdfs:comment>
    </owl:DatatypeProperty>
    


    <!-- http://www.hsu-ifa.de/ontologies/DINEN61360#Source_Document_of_Definition -->

    <owl:DatatypeProperty rdf:about="http://www.hsu-ifa.de/ontologies/DINEN61360#Source_Document_of_Definition">
        <rdfs:subPropertyOf rdf:resource="http://www.w3.org/2002/07/owl#topDataProperty"/>
        <rdfs:domain rdf:resource="http://www.hsu-ifa.de/ontologies/DINEN61360#Type_Description"/>
        <rdfs:comment>Description:
A link to a source file, where the definition of the data element was taken from

Liability: Optional

DIN EN 61360-1:2018 Section 8.6

Type: Should contain a description of the source document with a maximum of 80 characters. Document has to be approved by ISO or IEC (e.g. should be a standard like IEC XXXXX). Alternatively use a URL to give a source document that is not approved by ISO.

Poposed Data Range Expression: xsd:string</rdfs:comment>
    </owl:DatatypeProperty>
    


    <!-- http://www.hsu-ifa.de/ontologies/DINEN61360#Synonymous_Letter_Symbol -->

    <owl:DatatypeProperty rdf:about="http://www.hsu-ifa.de/ontologies/DINEN61360#Synonymous_Letter_Symbol">
        <rdfs:subPropertyOf rdf:resource="http://www.w3.org/2002/07/owl#topDataProperty"/>
        <rdfs:domain rdf:resource="http://www.hsu-ifa.de/ontologies/DINEN61360#Type_Description"/>
        <rdfs:comment>Description:
A synonym that is used for the preferred equation sign

Liability: Optional

DIN EN 61360-1:2018 Section 6.7

Type: IEC 60027, IEC 60747 or IEC 60148 compliant formula sign

Poposed Data Range Expression: xsd:string</rdfs:comment>
    </owl:DatatypeProperty>
    


    <!-- http://www.hsu-ifa.de/ontologies/DINEN61360#Synonymous_Name -->

    <owl:DatatypeProperty rdf:about="http://www.hsu-ifa.de/ontologies/DINEN61360#Synonymous_Name">
        <rdfs:subPropertyOf rdf:resource="http://www.w3.org/2002/07/owl#topDataProperty"/>
        <rdfs:domain rdf:resource="http://www.hsu-ifa.de/ontologies/DINEN61360#Type_Description"/>
        <rdfs:comment>Description:
Synonyms to the preferred name

Liability: Optional

DIN EN 61360-1:2018 Section 7.7

Type: String with lower and upper case, with a maximum of 70 characters

Poposed Data Range Expression: xsd:string[maxLength 70]</rdfs:comment>
    </owl:DatatypeProperty>
    


    <!-- http://www.hsu-ifa.de/ontologies/DINEN61360#Unit_of_Measure -->

    <owl:DatatypeProperty rdf:about="http://www.hsu-ifa.de/ontologies/DINEN61360#Unit_of_Measure">
        <rdfs:subPropertyOf rdf:resource="http://www.w3.org/2002/07/owl#topDataProperty"/>
        <rdfs:domain rdf:resource="http://www.hsu-ifa.de/ontologies/DINEN61360#Type_Description"/>
        <rdfs:comment>Description:
Defines the unit of measure for a data element (e.g. km/h)

Liability: case dependend, checked by SWRL rule 2

DIN EN 61360-1:2018 Section 10.7

Type: This data property represents the unit of measure, which should be ISO 31 compliant (SI-Units)

Poposed Data Range Expression: xsd:string</rdfs:comment>
    </owl:DatatypeProperty>
    


    <!-- http://www.hsu-ifa.de/ontologies/DINEN61360#Value -->

    <owl:DatatypeProperty rdf:about="http://www.hsu-ifa.de/ontologies/DINEN61360#Value">
        <rdfs:subPropertyOf rdf:resource="http://www.w3.org/2002/07/owl#topDataProperty"/>
        <rdf:type rdf:resource="http://www.w3.org/2002/07/owl#FunctionalProperty"/>
        <rdfs:domain>
            <owl:Class>
                <owl:intersectionOf rdf:parseType="Collection">
                    <rdf:Description rdf:about="http://www.hsu-ifa.de/ontologies/DINEN61360#Instance_Description"/>
                    <owl:Restriction>
                        <owl:onProperty rdf:resource="http://www.hsu-ifa.de/ontologies/DINEN61360#Instance_Description_has_Type"/>
                        <owl:allValuesFrom rdf:resource="http://www.hsu-ifa.de/ontologies/DINEN61360#Simple_Data_Type"/>
                    </owl:Restriction>
                </owl:intersectionOf>
            </owl:Class>
        </rdfs:domain>
        <rdfs:comment>Description:

The actual value of something being described.

Liability: Necessary

SemAnz40

Type: This data property represents the value of the data element, which is a string, while the actual data type is represented by the Data Property DataType (!)

Poposed Data Range Expression: xsd:string</rdfs:comment>
    </owl:DatatypeProperty>
    


    <!-- http://www.hsu-ifa.de/ontologies/DINEN61360#Value_Format_Field_length -->

    <owl:DatatypeProperty rdf:about="http://www.hsu-ifa.de/ontologies/DINEN61360#Value_Format_Field_length">
        <rdfs:subPropertyOf rdf:resource="http://www.w3.org/2002/07/owl#topDataProperty"/>
        <rdfs:domain rdf:resource="http://www.hsu-ifa.de/ontologies/DINEN61360#Type_Description"/>
        <rdfs:comment>Description:
Defines the representation of a data element in length and kind. See DIN61360 for detailed description of possible formats. Possible definitions include non-quantitative formats, quantitative formats and maximum count of characters

Liability: Necessary

DIN EN 61360-1:2018 Section 10.8

Type: This data property represents only the field length, since this could be exponential (expressed with an E), it is a string

Poposed Data Range Expression: xsd:string</rdfs:comment>
    </owl:DatatypeProperty>
    


    <!-- http://www.hsu-ifa.de/ontologies/DINEN61360#Value_Format_Field_length_Variable -->

    <owl:DatatypeProperty rdf:about="http://www.hsu-ifa.de/ontologies/DINEN61360#Value_Format_Field_length_Variable">
        <rdfs:subPropertyOf rdf:resource="http://www.w3.org/2002/07/owl#topDataProperty"/>
        <rdfs:domain rdf:resource="http://www.hsu-ifa.de/ontologies/DINEN61360#Type_Description"/>
        <rdfs:comment>Description:
Defines the representation of a data element in length and kind. See DIN61360 for detailed description of possible formats. Possible definitions include non-quantitative formats, quantitative formats and maximum count of characters

Liability: Necessary

DIN EN 61360-1:2018 Section 10.8

Type: This data property represents only the case, that a value format has a variable field length (true)

Poposed Data Range Expression: xsd:boolean</rdfs:comment>
    </owl:DatatypeProperty>
    


    <!-- http://www.hsu-ifa.de/ontologies/DINEN61360#Value_Format_non-quantitativ -->

    <owl:DatatypeProperty rdf:about="http://www.hsu-ifa.de/ontologies/DINEN61360#Value_Format_non-quantitativ">
        <rdfs:subPropertyOf rdf:resource="http://www.w3.org/2002/07/owl#topDataProperty"/>
        <rdfs:domain rdf:resource="http://www.hsu-ifa.de/ontologies/DINEN61360#Type_Description"/>
        <rdfs:range>
            <rdfs:Datatype>
                <owl:oneOf>
                    <rdf:Description>
                        <rdf:type rdf:resource="http://www.w3.org/1999/02/22-rdf-syntax-ns#List"/>
                        <rdf:first>A</rdf:first>
                        <rdf:rest>
                            <rdf:Description>
                                <rdf:type rdf:resource="http://www.w3.org/1999/02/22-rdf-syntax-ns#List"/>
                                <rdf:first>B</rdf:first>
                                <rdf:rest>
                                    <rdf:Description>
                                        <rdf:type rdf:resource="http://www.w3.org/1999/02/22-rdf-syntax-ns#List"/>
                                        <rdf:first>M</rdf:first>
                                        <rdf:rest>
                                            <rdf:Description>
                                                <rdf:type rdf:resource="http://www.w3.org/1999/02/22-rdf-syntax-ns#List"/>
                                                <rdf:first>N</rdf:first>
                                                <rdf:rest>
                                                    <rdf:Description>
                                                        <rdf:type rdf:resource="http://www.w3.org/1999/02/22-rdf-syntax-ns#List"/>
                                                        <rdf:first>X</rdf:first>
                                                        <rdf:rest rdf:resource="http://www.w3.org/1999/02/22-rdf-syntax-ns#nil"/>
                                                    </rdf:Description>
                                                </rdf:rest>
                                            </rdf:Description>
                                        </rdf:rest>
                                    </rdf:Description>
                                </rdf:rest>
                            </rdf:Description>
                        </rdf:rest>
                    </rdf:Description>
                </owl:oneOf>
            </rdfs:Datatype>
        </rdfs:range>
        <owl:propertyDisjointWith rdf:resource="http://www.hsu-ifa.de/ontologies/DINEN61360#Value_Format_quantitativ"/>
        <rdfs:comment>Description:
Defines the representation of a data element in length and kind. See DIN61360 for detailed description of possible formats. Possible definitions include non-quantitative formats, quantitative formats and maximum count of characters

Liability: Necessary

DIN EN 61360-1:2018 Section 10.8

Type: This data property represents only the non-quantitativ formats, string

Poposed Data Range Expression: xsd:string</rdfs:comment>
    </owl:DatatypeProperty>
    


    <!-- http://www.hsu-ifa.de/ontologies/DINEN61360#Value_Format_quantitativ -->

    <owl:DatatypeProperty rdf:about="http://www.hsu-ifa.de/ontologies/DINEN61360#Value_Format_quantitativ">
        <rdfs:subPropertyOf rdf:resource="http://www.w3.org/2002/07/owl#topDataProperty"/>
        <rdfs:domain rdf:resource="http://www.hsu-ifa.de/ontologies/DINEN61360#Type_Description"/>
        <rdfs:range>
            <rdfs:Datatype>
                <owl:oneOf>
                    <rdf:Description>
                        <rdf:type rdf:resource="http://www.w3.org/1999/02/22-rdf-syntax-ns#List"/>
                        <rdf:first>NR1</rdf:first>
                        <rdf:rest>
                            <rdf:Description>
                                <rdf:type rdf:resource="http://www.w3.org/1999/02/22-rdf-syntax-ns#List"/>
                                <rdf:first>NR2</rdf:first>
                                <rdf:rest>
                                    <rdf:Description>
                                        <rdf:type rdf:resource="http://www.w3.org/1999/02/22-rdf-syntax-ns#List"/>
                                        <rdf:first>NR3</rdf:first>
                                        <rdf:rest rdf:resource="http://www.w3.org/1999/02/22-rdf-syntax-ns#nil"/>
                                    </rdf:Description>
                                </rdf:rest>
                            </rdf:Description>
                        </rdf:rest>
                    </rdf:Description>
                </owl:oneOf>
            </rdfs:Datatype>
        </rdfs:range>
        <rdfs:comment>Description:
Defines the representation of a data element in length and kind. See DIN61360 for detailed description of possible formats. Possible definitions include non-quantitative formats, quantitative formats and maximum count of characters

Liability: Necessary

DIN EN 61360-1:2018 Section 10.8

Type: This data property represents only the quantitativ formats, string

Poposed Data Range Expression: xsd:string</rdfs:comment>
    </owl:DatatypeProperty>
    


    <!-- http://www.hsu-ifa.de/ontologies/DINEN61360#Value_List -->

    <owl:DatatypeProperty rdf:about="http://www.hsu-ifa.de/ontologies/DINEN61360#Value_List">
        <rdfs:subPropertyOf rdf:resource="http://www.w3.org/2002/07/owl#topDataProperty"/>
        <rdfs:domain rdf:resource="http://www.hsu-ifa.de/ontologies/DINEN61360#Simple_Data_Type"/>
        <rdfs:comment>Description: 
Represents the possible values for a data element

Liability: optional (in DIN613060 case depended due to classification of data element, which is not implemented here)

DIN EN 61360-1:2018 Section 16

Type: This data property represents the information, if there is a value list (if so, true), basically the values that the data property &quot;Value&quot; is allowed to hold. 

Poposed Data Range Expression: xsd:boolean</rdfs:comment>
    </owl:DatatypeProperty>
    


    <!-- http://www.hsu-ifa.de/ontologies/DINEN61360#Value_List_Member -->

    <owl:DatatypeProperty rdf:about="http://www.hsu-ifa.de/ontologies/DINEN61360#Value_List_Member">
        <rdfs:subPropertyOf rdf:resource="http://www.w3.org/2002/07/owl#topDataProperty"/>
        <rdfs:domain rdf:resource="http://www.hsu-ifa.de/ontologies/DINEN61360#Simple_Data_Type"/>
        <rdfs:comment>Description: 
Represents the possible values for a data element

Liability: optional (in DIN613060 case depended due to classification of data element, which is not implemented here)

DIN EN 61360-1:2018 Section 16

Type: This data property represents the one (!) member of the value list, violation may result in inconsistency, since the compliance of value list and value is checked by SWRL rule 3. 

Poposed Data Range Expression: xsd:string</rdfs:comment>
    </owl:DatatypeProperty>
    


    <!-- http://www.hsu-ifa.de/ontologies/DINEN61360#Version_Number -->

    <owl:DatatypeProperty rdf:about="http://www.hsu-ifa.de/ontologies/DINEN61360#Version_Number">
        <rdfs:subPropertyOf rdf:resource="http://www.w3.org/2002/07/owl#topDataProperty"/>
        <rdfs:domain rdf:resource="http://www.hsu-ifa.de/ontologies/DINEN61360#Type_Description"/>
        <rdfs:comment>Description:
Number that indicates different versions of one data element type

Liability: Necessary

DIN EN 61360-1:2018 Section 7.8

Type: Integer with three digits max, so between 1 and 999

Poposed Data Range Expression: xsd:integer[&gt;= 1 , &lt;= 999]</rdfs:comment>
    </owl:DatatypeProperty>
    


    <!-- http://www.hsu-ifa.de/ontologies/DINEN61360#backwards_compatible_Revision -->

    <owl:DatatypeProperty rdf:about="http://www.hsu-ifa.de/ontologies/DINEN61360#backwards_compatible_Revision">
        <rdfs:domain rdf:resource="http://www.hsu-ifa.de/ontologies/DINEN61360#Type_Description"/>
        <rdfs:comment>Description:
Indicates, to which revisions the data type is backwards compatible.

Type: Integer

Poposed Data Range Expression: xsd:string</rdfs:comment>
    </owl:DatatypeProperty>
    


    <!-- http://www.hsu-ifa.de/ontologies/DINEN61360#backwards_compatible_Version -->

    <owl:DatatypeProperty rdf:about="http://www.hsu-ifa.de/ontologies/DINEN61360#backwards_compatible_Version">
        <rdfs:domain rdf:resource="http://www.hsu-ifa.de/ontologies/DINEN61360#Type_Description"/>
        <rdfs:comment>Description:
Indicates, to which version numbers the data type is backwards compatible.

Type: Integer

Poposed Data Range Expression: xsd:string</rdfs:comment>
    </owl:DatatypeProperty>
    


    <!-- http://www.hsu-ifa.de/ontologies/VDI3682#longName -->

    <owl:DatatypeProperty rdf:about="http://www.hsu-ifa.de/ontologies/VDI3682#longName">
        <rdf:type rdf:resource="http://www.w3.org/2002/07/owl#FunctionalProperty"/>
        <rdfs:comment>A property that is used to give a long name to an individual.</rdfs:comment>
    </owl:DatatypeProperty>
    


    <!-- http://www.hsu-ifa.de/ontologies/VDI3682#shortName -->

    <owl:DatatypeProperty rdf:about="http://www.hsu-ifa.de/ontologies/VDI3682#shortName">
        <rdf:type rdf:resource="http://www.w3.org/2002/07/owl#FunctionalProperty"/>
        <rdfs:comment>A property that is used to give a short name to an individual.</rdfs:comment>
    </owl:DatatypeProperty>
    


    <!-- 
    ///////////////////////////////////////////////////////////////////////////////////////
    //
    // Classes
    //
    ///////////////////////////////////////////////////////////////////////////////////////
     -->

    


    <!-- http://www.hsu-hh.de/aut/ontologies/agent-summer-school#Agent -->

    <owl:Class rdf:about="http://www.hsu-hh.de/aut/ontologies/agent-summer-school#Agent"/>
    


    <!-- http://www.hsu-hh.de/aut/ontologies/agent-summer-school#Capability -->

    <owl:Class rdf:about="http://www.hsu-hh.de/aut/ontologies/agent-summer-school#Capability">
        <owl:equivalentClass rdf:resource="http://www.hsu-ifa.de/ontologies/VDI3682#ProcessOperator"/>
    </owl:Class>
    


    <!-- http://www.hsu-hh.de/aut/ontologies/agent-summer-school#ConveyorAgent -->

    <owl:Class rdf:about="http://www.hsu-hh.de/aut/ontologies/agent-summer-school#ConveyorAgent">
        <rdfs:subClassOf rdf:resource="http://www.hsu-hh.de/aut/ontologies/agent-summer-school#Agent"/>
    </owl:Class>
    


    <!-- http://www.hsu-hh.de/aut/ontologies/agent-summer-school#DetectProduct -->

    <owl:Class rdf:about="http://www.hsu-hh.de/aut/ontologies/agent-summer-school#DetectProduct">
        <rdfs:subClassOf rdf:resource="http://www.hsu-hh.de/aut/ontologies/agent-summer-school#Capability"/>
    </owl:Class>
    


    <!-- http://www.hsu-hh.de/aut/ontologies/agent-summer-school#GripperAgent -->

    <owl:Class rdf:about="http://www.hsu-hh.de/aut/ontologies/agent-summer-school#GripperAgent">
        <rdfs:subClassOf rdf:resource="http://www.hsu-hh.de/aut/ontologies/agent-summer-school#Agent"/>
    </owl:Class>
    


    <!-- http://www.hsu-hh.de/aut/ontologies/agent-summer-school#Handling -->

    <owl:Class rdf:about="http://www.hsu-hh.de/aut/ontologies/agent-summer-school#Handling">
        <rdfs:subClassOf rdf:resource="http://www.hsu-hh.de/aut/ontologies/agent-summer-school#Capability"/>
    </owl:Class>
    


    <!-- http://www.hsu-hh.de/aut/ontologies/agent-summer-school#MeasureProductLength -->

    <owl:Class rdf:about="http://www.hsu-hh.de/aut/ontologies/agent-summer-school#MeasureProductLength">
        <rdfs:subClassOf rdf:resource="http://www.hsu-hh.de/aut/ontologies/agent-summer-school#Capability"/>
    </owl:Class>
    


    <!-- http://www.hsu-hh.de/aut/ontologies/agent-summer-school#Product -->

    <owl:Class rdf:about="http://www.hsu-hh.de/aut/ontologies/agent-summer-school#Product"/>
    


    <!-- http://www.hsu-hh.de/aut/ontologies/agent-summer-school#SensorAgent -->

    <owl:Class rdf:about="http://www.hsu-hh.de/aut/ontologies/agent-summer-school#SensorAgent">
        <rdfs:subClassOf rdf:resource="http://www.hsu-hh.de/aut/ontologies/agent-summer-school#Agent"/>
    </owl:Class>
    


    <!-- http://www.hsu-hh.de/aut/ontologies/agent-summer-school#Transport -->

    <owl:Class rdf:about="http://www.hsu-hh.de/aut/ontologies/agent-summer-school#Transport">
        <rdfs:subClassOf rdf:resource="http://www.hsu-hh.de/aut/ontologies/agent-summer-school#Capability"/>
    </owl:Class>
    


    <!-- http://www.hsu-ifa.de/ontologies/DINEN61360#Array -->

    <owl:Class rdf:about="http://www.hsu-ifa.de/ontologies/DINEN61360#Array">
        <rdfs:subClassOf rdf:resource="http://www.hsu-ifa.de/ontologies/DINEN61360#Complex_Data_Type"/>
        <rdfs:subClassOf>
            <owl:Restriction>
                <owl:onProperty rdf:resource="http://www.hsu-ifa.de/ontologies/DINEN61360#complex_Data_Type_has_Member"/>
                <owl:allValuesFrom rdf:resource="http://www.hsu-ifa.de/ontologies/DINEN61360#Array_Member"/>
            </owl:Restriction>
        </rdfs:subClassOf>
    </owl:Class>
    


    <!-- http://www.hsu-ifa.de/ontologies/DINEN61360#Array_Member -->

    <owl:Class rdf:about="http://www.hsu-ifa.de/ontologies/DINEN61360#Array_Member">
        <rdfs:subClassOf rdf:resource="http://www.hsu-ifa.de/ontologies/DINEN61360#Complex_Data_Type_Member"/>
        <rdfs:subClassOf>
            <owl:Restriction>
                <owl:onProperty rdf:resource="http://www.hsu-ifa.de/ontologies/DINEN61360#Array_Member_Dimension"/>
                <owl:qualifiedCardinality rdf:datatype="http://www.w3.org/2001/XMLSchema#nonNegativeInteger">1</owl:qualifiedCardinality>
                <owl:onDataRange rdf:resource="http://www.w3.org/2001/XMLSchema#int"/>
            </owl:Restriction>
        </rdfs:subClassOf>
        <rdfs:subClassOf>
            <owl:Restriction>
                <owl:onProperty rdf:resource="http://www.hsu-ifa.de/ontologies/DINEN61360#Array_Member_Position"/>
                <owl:qualifiedCardinality rdf:datatype="http://www.w3.org/2001/XMLSchema#nonNegativeInteger">1</owl:qualifiedCardinality>
                <owl:onDataRange rdf:resource="http://www.w3.org/2001/XMLSchema#int"/>
            </owl:Restriction>
        </rdfs:subClassOf>
    </owl:Class>
    


    <!-- http://www.hsu-ifa.de/ontologies/DINEN61360#Bag -->

    <owl:Class rdf:about="http://www.hsu-ifa.de/ontologies/DINEN61360#Bag">
        <rdfs:subClassOf rdf:resource="http://www.hsu-ifa.de/ontologies/DINEN61360#Complex_Data_Type"/>
        <rdfs:subClassOf>
            <owl:Restriction>
                <owl:onProperty rdf:resource="http://www.hsu-ifa.de/ontologies/DINEN61360#complex_Data_Type_has_Member"/>
                <owl:allValuesFrom rdf:resource="http://www.hsu-ifa.de/ontologies/DINEN61360#Bag_Member"/>
            </owl:Restriction>
        </rdfs:subClassOf>
    </owl:Class>
    


    <!-- http://www.hsu-ifa.de/ontologies/DINEN61360#Bag_Member -->

    <owl:Class rdf:about="http://www.hsu-ifa.de/ontologies/DINEN61360#Bag_Member">
        <rdfs:subClassOf rdf:resource="http://www.hsu-ifa.de/ontologies/DINEN61360#Complex_Data_Type_Member"/>
    </owl:Class>
    


    <!-- http://www.hsu-ifa.de/ontologies/DINEN61360#Boolean -->

    <owl:Class rdf:about="http://www.hsu-ifa.de/ontologies/DINEN61360#Boolean">
        <rdfs:subClassOf rdf:resource="http://www.hsu-ifa.de/ontologies/DINEN61360#Simple_Data_Type"/>
        <rdfs:subClassOf>
            <owl:Restriction>
                <owl:onProperty rdf:resource="http://www.hsu-ifa.de/ontologies/DINEN61360#Value_List_Member"/>
                <owl:allValuesFrom rdf:resource="http://www.w3.org/2001/XMLSchema#boolean"/>
            </owl:Restriction>
        </rdfs:subClassOf>
    </owl:Class>
    


    <!-- http://www.hsu-ifa.de/ontologies/DINEN61360#Complex_Data_Type -->

    <owl:Class rdf:about="http://www.hsu-ifa.de/ontologies/DINEN61360#Complex_Data_Type">
        <rdfs:subClassOf rdf:resource="http://www.hsu-ifa.de/ontologies/DINEN61360#Data_Type"/>
        <owl:disjointWith rdf:resource="http://www.hsu-ifa.de/ontologies/DINEN61360#Simple_Data_Type"/>
    </owl:Class>
    


    <!-- http://www.hsu-ifa.de/ontologies/DINEN61360#Complex_Data_Type_Member -->

    <owl:Class rdf:about="http://www.hsu-ifa.de/ontologies/DINEN61360#Complex_Data_Type_Member">
        <rdfs:subClassOf rdf:resource="http://www.hsu-ifa.de/ontologies/DINEN61360#Data_Type"/>
    </owl:Class>
    


    <!-- http://www.hsu-ifa.de/ontologies/DINEN61360#Data_Element -->

    <owl:Class rdf:about="http://www.hsu-ifa.de/ontologies/DINEN61360#Data_Element">
        <rdfs:subClassOf>
            <owl:Class>
                <owl:intersectionOf rdf:parseType="Collection">
                    <owl:Restriction>
                        <owl:onProperty rdf:resource="http://www.hsu-ifa.de/ontologies/DINEN61360#has_Instance_Description"/>
                        <owl:maxQualifiedCardinality rdf:datatype="http://www.w3.org/2001/XMLSchema#nonNegativeInteger">1</owl:maxQualifiedCardinality>
                        <owl:onClass>
                            <owl:Class>
                                <owl:intersectionOf rdf:parseType="Collection">
                                    <rdf:Description rdf:about="http://www.hsu-ifa.de/ontologies/DINEN61360#Instance_Description"/>
                                    <owl:Restriction>
                                        <owl:onProperty rdf:resource="http://www.hsu-ifa.de/ontologies/DINEN61360#Expression_Goal"/>
                                        <owl:hasValue>Actual_Value</owl:hasValue>
                                    </owl:Restriction>
                                </owl:intersectionOf>
                            </owl:Class>
                        </owl:onClass>
                    </owl:Restriction>
                    <owl:Restriction>
                        <owl:onProperty rdf:resource="http://www.hsu-ifa.de/ontologies/DINEN61360#has_Instance_Description"/>
                        <owl:maxQualifiedCardinality rdf:datatype="http://www.w3.org/2001/XMLSchema#nonNegativeInteger">1</owl:maxQualifiedCardinality>
                        <owl:onClass>
                            <owl:Class>
                                <owl:intersectionOf rdf:parseType="Collection">
                                    <rdf:Description rdf:about="http://www.hsu-ifa.de/ontologies/DINEN61360#Instance_Description"/>
                                    <owl:Restriction>
                                        <owl:onProperty rdf:resource="http://www.hsu-ifa.de/ontologies/DINEN61360#Expression_Goal"/>
                                        <owl:hasValue>Assurance</owl:hasValue>
                                    </owl:Restriction>
                                </owl:intersectionOf>
                            </owl:Class>
                        </owl:onClass>
                    </owl:Restriction>
                    <owl:Restriction>
                        <owl:onProperty rdf:resource="http://www.hsu-ifa.de/ontologies/DINEN61360#has_Instance_Description"/>
                        <owl:maxQualifiedCardinality rdf:datatype="http://www.w3.org/2001/XMLSchema#nonNegativeInteger">1</owl:maxQualifiedCardinality>
                        <owl:onClass>
                            <owl:Class>
                                <owl:intersectionOf rdf:parseType="Collection">
                                    <rdf:Description rdf:about="http://www.hsu-ifa.de/ontologies/DINEN61360#Instance_Description"/>
                                    <owl:Restriction>
                                        <owl:onProperty rdf:resource="http://www.hsu-ifa.de/ontologies/DINEN61360#Expression_Goal"/>
                                        <owl:hasValue>Requirement</owl:hasValue>
                                    </owl:Restriction>
                                </owl:intersectionOf>
                            </owl:Class>
                        </owl:onClass>
                    </owl:Restriction>
                </owl:intersectionOf>
            </owl:Class>
        </rdfs:subClassOf>
        <rdfs:subClassOf>
            <owl:Restriction>
                <owl:onProperty rdf:resource="http://www.hsu-ifa.de/ontologies/DINEN61360#has_Type_Description"/>
                <owl:someValuesFrom rdf:resource="http://www.hsu-ifa.de/ontologies/DINEN61360#Type_Description"/>
            </owl:Restriction>
        </rdfs:subClassOf>
        <rdfs:subClassOf>
            <owl:Restriction>
                <owl:onProperty rdf:resource="http://www.hsu-ifa.de/ontologies/DINEN61360#has_Instance_Description"/>
                <owl:minQualifiedCardinality rdf:datatype="http://www.w3.org/2001/XMLSchema#nonNegativeInteger">0</owl:minQualifiedCardinality>
                <owl:onClass rdf:resource="http://www.hsu-ifa.de/ontologies/DINEN61360#Instance_Description"/>
            </owl:Restriction>
        </rdfs:subClassOf>
        <owl:disjointWith rdf:resource="http://www.hsu-ifa.de/ontologies/DINEN61360#Type_Description"/>
        <rdfs:comment>Description:
Contains a the structure of all data element (DIN61360 3.5.2, see also section 4)

Each Data_Element has to have a type description and may have an instance description</rdfs:comment>
    </owl:Class>
    


    <!-- http://www.hsu-ifa.de/ontologies/DINEN61360#Data_Type -->

    <owl:Class rdf:about="http://www.hsu-ifa.de/ontologies/DINEN61360#Data_Type"/>
    


    <!-- http://www.hsu-ifa.de/ontologies/DINEN61360#Instance_Description -->

    <owl:Class rdf:about="http://www.hsu-ifa.de/ontologies/DINEN61360#Instance_Description">
        <rdfs:subClassOf>
            <owl:Restriction>
                <owl:onProperty rdf:resource="http://www.hsu-ifa.de/ontologies/DINEN61360#Expression_Goal"/>
                <owl:qualifiedCardinality rdf:datatype="http://www.w3.org/2001/XMLSchema#nonNegativeInteger">1</owl:qualifiedCardinality>
                <owl:onDataRange rdf:resource="http://www.w3.org/2001/XMLSchema#string"/>
            </owl:Restriction>
        </rdfs:subClassOf>
        <rdfs:subClassOf>
            <owl:Restriction>
                <owl:onProperty rdf:resource="http://www.hsu-ifa.de/ontologies/DINEN61360#Logic_Interpretation"/>
                <owl:qualifiedCardinality rdf:datatype="http://www.w3.org/2001/XMLSchema#nonNegativeInteger">1</owl:qualifiedCardinality>
                <owl:onDataRange rdf:resource="http://www.w3.org/2001/XMLSchema#string"/>
            </owl:Restriction>
        </rdfs:subClassOf>
        <owl:disjointWith rdf:resource="http://www.hsu-ifa.de/ontologies/DINEN61360#Type_Description"/>
    </owl:Class>
    


    <!-- http://www.hsu-ifa.de/ontologies/DINEN61360#Integer -->

    <owl:Class rdf:about="http://www.hsu-ifa.de/ontologies/DINEN61360#Integer">
        <rdfs:subClassOf rdf:resource="http://www.hsu-ifa.de/ontologies/DINEN61360#Simple_Data_Type"/>
        <rdfs:subClassOf>
            <owl:Restriction>
                <owl:onProperty rdf:resource="http://www.hsu-ifa.de/ontologies/DINEN61360#Value_List_Member"/>
                <owl:allValuesFrom rdf:resource="http://www.w3.org/2001/XMLSchema#int"/>
            </owl:Restriction>
        </rdfs:subClassOf>
    </owl:Class>
    


    <!-- http://www.hsu-ifa.de/ontologies/DINEN61360#List -->

    <owl:Class rdf:about="http://www.hsu-ifa.de/ontologies/DINEN61360#List">
        <rdfs:subClassOf rdf:resource="http://www.hsu-ifa.de/ontologies/DINEN61360#Complex_Data_Type"/>
        <rdfs:subClassOf>
            <owl:Restriction>
                <owl:onProperty rdf:resource="http://www.hsu-ifa.de/ontologies/DINEN61360#complex_Data_Type_has_Member"/>
                <owl:allValuesFrom rdf:resource="http://www.hsu-ifa.de/ontologies/DINEN61360#List_Member"/>
            </owl:Restriction>
        </rdfs:subClassOf>
    </owl:Class>
    


    <!-- http://www.hsu-ifa.de/ontologies/DINEN61360#List_Member -->

    <owl:Class rdf:about="http://www.hsu-ifa.de/ontologies/DINEN61360#List_Member">
        <rdfs:subClassOf rdf:resource="http://www.hsu-ifa.de/ontologies/DINEN61360#Complex_Data_Type_Member"/>
        <rdfs:subClassOf>
            <owl:Restriction>
                <owl:onProperty rdf:resource="http://www.hsu-ifa.de/ontologies/DINEN61360#List_Member_Position"/>
                <owl:qualifiedCardinality rdf:datatype="http://www.w3.org/2001/XMLSchema#nonNegativeInteger">1</owl:qualifiedCardinality>
                <owl:onDataRange rdf:resource="http://www.w3.org/2001/XMLSchema#int"/>
            </owl:Restriction>
        </rdfs:subClassOf>
    </owl:Class>
    


    <!-- http://www.hsu-ifa.de/ontologies/DINEN61360#Real -->

    <owl:Class rdf:about="http://www.hsu-ifa.de/ontologies/DINEN61360#Real">
        <rdfs:subClassOf rdf:resource="http://www.hsu-ifa.de/ontologies/DINEN61360#Simple_Data_Type"/>
        <rdfs:subClassOf>
            <owl:Restriction>
                <owl:onProperty rdf:resource="http://www.hsu-ifa.de/ontologies/DINEN61360#Value_List_Member"/>
                <owl:allValuesFrom rdf:resource="http://www.w3.org/2001/XMLSchema#float"/>
            </owl:Restriction>
        </rdfs:subClassOf>
    </owl:Class>
    


    <!-- http://www.hsu-ifa.de/ontologies/DINEN61360#Set -->

    <owl:Class rdf:about="http://www.hsu-ifa.de/ontologies/DINEN61360#Set">
        <rdfs:subClassOf rdf:resource="http://www.hsu-ifa.de/ontologies/DINEN61360#Complex_Data_Type"/>
        <rdfs:subClassOf>
            <owl:Restriction>
                <owl:onProperty rdf:resource="http://www.hsu-ifa.de/ontologies/DINEN61360#complex_Data_Type_has_Member"/>
                <owl:allValuesFrom rdf:resource="http://www.hsu-ifa.de/ontologies/DINEN61360#Set_Member"/>
            </owl:Restriction>
        </rdfs:subClassOf>
    </owl:Class>
    


    <!-- http://www.hsu-ifa.de/ontologies/DINEN61360#Set_Member -->

    <owl:Class rdf:about="http://www.hsu-ifa.de/ontologies/DINEN61360#Set_Member">
        <rdfs:subClassOf rdf:resource="http://www.hsu-ifa.de/ontologies/DINEN61360#Complex_Data_Type_Member"/>
    </owl:Class>
    


    <!-- http://www.hsu-ifa.de/ontologies/DINEN61360#Simple_Data_Type -->

    <owl:Class rdf:about="http://www.hsu-ifa.de/ontologies/DINEN61360#Simple_Data_Type">
        <rdfs:subClassOf rdf:resource="http://www.hsu-ifa.de/ontologies/DINEN61360#Data_Type"/>
        <rdfs:subClassOf>
            <owl:Restriction>
                <owl:onProperty rdf:resource="http://www.hsu-ifa.de/ontologies/DINEN61360#Value_List"/>
                <owl:qualifiedCardinality rdf:datatype="http://www.w3.org/2001/XMLSchema#nonNegativeInteger">1</owl:qualifiedCardinality>
                <owl:onDataRange rdf:resource="http://www.w3.org/2001/XMLSchema#boolean"/>
            </owl:Restriction>
        </rdfs:subClassOf>
        <rdfs:comment>Description:
Indicates which kind of DataType a data element must be. This does not include all data types of DIN61360! 

Liability: Necessary

DIN61360: 3.4.1

Type: is a enumeration of standard compliant data types. Please see DIN61360 for a description of level/class-instance/list/set/bag/array</rdfs:comment>
    </owl:Class>
    


    <!-- http://www.hsu-ifa.de/ontologies/DINEN61360#String -->

    <owl:Class rdf:about="http://www.hsu-ifa.de/ontologies/DINEN61360#String">
        <rdfs:subClassOf rdf:resource="http://www.hsu-ifa.de/ontologies/DINEN61360#Simple_Data_Type"/>
        <rdfs:subClassOf>
            <owl:Restriction>
                <owl:onProperty rdf:resource="http://www.hsu-ifa.de/ontologies/DINEN61360#Value_List_Member"/>
                <owl:allValuesFrom rdf:resource="http://www.w3.org/2001/XMLSchema#string"/>
            </owl:Restriction>
        </rdfs:subClassOf>
    </owl:Class>
    


    <!-- http://www.hsu-ifa.de/ontologies/DINEN61360#Type_Description -->

    <owl:Class rdf:about="http://www.hsu-ifa.de/ontologies/DINEN61360#Type_Description">
        <rdfs:subClassOf>
            <owl:Restriction>
                <owl:onProperty rdf:resource="http://www.hsu-ifa.de/ontologies/DINEN61360#Code"/>
                <owl:qualifiedCardinality rdf:datatype="http://www.w3.org/2001/XMLSchema#nonNegativeInteger">1</owl:qualifiedCardinality>
                <owl:onDataRange rdf:resource="http://www.w3.org/2001/XMLSchema#string"/>
            </owl:Restriction>
        </rdfs:subClassOf>
        <rdfs:subClassOf>
            <owl:Restriction>
                <owl:onProperty rdf:resource="http://www.hsu-ifa.de/ontologies/DINEN61360#Definition"/>
                <owl:qualifiedCardinality rdf:datatype="http://www.w3.org/2001/XMLSchema#nonNegativeInteger">1</owl:qualifiedCardinality>
                <owl:onDataRange rdf:resource="http://www.w3.org/2001/XMLSchema#string"/>
            </owl:Restriction>
        </rdfs:subClassOf>
        <rdfs:subClassOf>
            <owl:Restriction>
                <owl:onProperty rdf:resource="http://www.hsu-ifa.de/ontologies/DINEN61360#Preferred_Name"/>
                <owl:qualifiedCardinality rdf:datatype="http://www.w3.org/2001/XMLSchema#nonNegativeInteger">1</owl:qualifiedCardinality>
                <owl:onDataRange rdf:resource="http://www.w3.org/2001/XMLSchema#string"/>
            </owl:Restriction>
        </rdfs:subClassOf>
        <rdfs:subClassOf>
            <owl:Restriction>
                <owl:onProperty rdf:resource="http://www.hsu-ifa.de/ontologies/DINEN61360#Short_Name"/>
                <owl:qualifiedCardinality rdf:datatype="http://www.w3.org/2001/XMLSchema#nonNegativeInteger">1</owl:qualifiedCardinality>
                <owl:onDataRange rdf:resource="http://www.w3.org/2001/XMLSchema#string"/>
            </owl:Restriction>
        </rdfs:subClassOf>
        <rdfs:subClassOf>
            <owl:Restriction>
                <owl:onProperty rdf:resource="http://www.hsu-ifa.de/ontologies/DINEN61360#Version_Number"/>
                <owl:qualifiedCardinality rdf:datatype="http://www.w3.org/2001/XMLSchema#nonNegativeInteger">1</owl:qualifiedCardinality>
                <owl:onDataRange rdf:resource="http://www.w3.org/2001/XMLSchema#int"/>
            </owl:Restriction>
        </rdfs:subClassOf>
        <rdfs:subClassOf>
            <owl:Restriction>
                <owl:onProperty rdf:resource="http://www.hsu-ifa.de/ontologies/DINEN61360#Preferred_Letter_Symbol"/>
                <owl:maxQualifiedCardinality rdf:datatype="http://www.w3.org/2001/XMLSchema#nonNegativeInteger">1</owl:maxQualifiedCardinality>
                <owl:onDataRange rdf:resource="http://www.w3.org/2001/XMLSchema#string"/>
            </owl:Restriction>
        </rdfs:subClassOf>
        <rdfs:subClassOf>
            <owl:Restriction>
                <owl:onProperty rdf:resource="http://www.hsu-ifa.de/ontologies/DINEN61360#Synonymous_Letter_Symbol"/>
                <owl:maxQualifiedCardinality rdf:datatype="http://www.w3.org/2001/XMLSchema#nonNegativeInteger">2</owl:maxQualifiedCardinality>
                <owl:onDataRange rdf:resource="http://www.w3.org/2001/XMLSchema#string"/>
            </owl:Restriction>
        </rdfs:subClassOf>
        <rdfs:subClassOf>
            <owl:Restriction>
                <owl:onProperty rdf:resource="http://www.hsu-ifa.de/ontologies/DINEN61360#Synonymous_Name"/>
                <owl:maxQualifiedCardinality rdf:datatype="http://www.w3.org/2001/XMLSchema#nonNegativeInteger">2</owl:maxQualifiedCardinality>
                <owl:onDataRange rdf:resource="http://www.w3.org/2001/XMLSchema#string"/>
            </owl:Restriction>
        </rdfs:subClassOf>
        <rdfs:comment>Value list is expressed as exactly 1, since not using a value list has to result in value list false</rdfs:comment>
    </owl:Class>
    


    <!-- http://www.hsu-ifa.de/ontologies/VDI3682#Energy -->

    <owl:Class rdf:about="http://www.hsu-ifa.de/ontologies/VDI3682#Energy">
        <rdfs:subClassOf rdf:resource="http://www.hsu-ifa.de/ontologies/VDI3682#State"/>
        <rdfs:comment>Energy is requiered by the process operator to fullfill the process. Energy is Input and Output of a process. Energy can be any kind of energy, exp.: electricity, heat,...</rdfs:comment>
    </owl:Class>
    


    <!-- http://www.hsu-ifa.de/ontologies/VDI3682#Information -->

    <owl:Class rdf:about="http://www.hsu-ifa.de/ontologies/VDI3682#Information">
        <rdfs:subClassOf rdf:resource="http://www.hsu-ifa.de/ontologies/VDI3682#State"/>
        <rdfs:comment>Information input for a process operator can be any kind of information required to fullfill the process. Information output can be any kind of information created by the process.
[VDI 3682-1]</rdfs:comment>
    </owl:Class>
    


    <!-- http://www.hsu-ifa.de/ontologies/VDI3682#Process -->

    <owl:Class rdf:about="http://www.hsu-ifa.de/ontologies/VDI3682#Process">
        <owl:disjointWith rdf:resource="http://www.hsu-ifa.de/ontologies/VDI3682#State"/>
        <owl:disjointWith rdf:resource="http://www.hsu-ifa.de/ontologies/VDI3682#SystemLimit"/>
        <owl:disjointWith rdf:resource="http://www.hsu-ifa.de/ontologies/VDI3682#TechnicalResource"/>
        <rdfs:comment>A process describes the desired behavior of a process operator, by means of a solution neutral description of inputs and outputs. Products,energies  and information are converted into new products,energies  and information by a process operator. The process operator implements this conversion with the help of technical resources.
[VDI3682-1]

Note that a process may have inputs and outputs. These are inputs / outputs that are on the system limit of this process.</rdfs:comment>
    </owl:Class>
    


    <!-- http://www.hsu-ifa.de/ontologies/VDI3682#ProcessOperator -->

    <owl:Class rdf:about="http://www.hsu-ifa.de/ontologies/VDI3682#ProcessOperator">
        <owl:equivalentClass>
            <owl:Class>
                <owl:intersectionOf rdf:parseType="Collection">
                    <owl:Restriction>
                        <owl:onProperty rdf:resource="http://www.hsu-ifa.de/ontologies/VDI3682#hasInput"/>
                        <owl:someValuesFrom rdf:resource="http://www.w3.org/2002/07/owl#Thing"/>
                    </owl:Restriction>
                    <owl:Restriction>
                        <owl:onProperty rdf:resource="http://www.hsu-ifa.de/ontologies/VDI3682#hasOutput"/>
                        <owl:someValuesFrom rdf:resource="http://www.w3.org/2002/07/owl#Thing"/>
                    </owl:Restriction>
                    <owl:Restriction>
                        <owl:onProperty>
                            <rdf:Description>
                                <owl:inverseOf rdf:resource="http://www.hsu-ifa.de/ontologies/VDI3682#consistsOf"/>
                            </rdf:Description>
                        </owl:onProperty>
                        <owl:someValuesFrom rdf:resource="http://www.hsu-ifa.de/ontologies/VDI3682#Process"/>
                    </owl:Restriction>
                </owl:intersectionOf>
            </owl:Class>
        </owl:equivalentClass>
        <rdfs:subClassOf>
            <owl:Class>
                <owl:intersectionOf rdf:parseType="Collection">
                    <owl:Restriction>
                        <owl:onProperty rdf:resource="http://www.hsu-ifa.de/ontologies/VDI3682#hasInput"/>
                        <owl:someValuesFrom rdf:resource="http://www.w3.org/2002/07/owl#Thing"/>
                    </owl:Restriction>
                    <owl:Restriction>
                        <owl:onProperty rdf:resource="http://www.hsu-ifa.de/ontologies/VDI3682#hasOutput"/>
                        <owl:someValuesFrom rdf:resource="http://www.w3.org/2002/07/owl#Thing"/>
                    </owl:Restriction>
                </owl:intersectionOf>
            </owl:Class>
        </rdfs:subClassOf>
        <owl:disjointWith rdf:resource="http://www.hsu-ifa.de/ontologies/VDI3682#State"/>
        <owl:disjointWith rdf:resource="http://www.hsu-ifa.de/ontologies/VDI3682#SystemLimit"/>
        <owl:disjointWith rdf:resource="http://www.hsu-ifa.de/ontologies/VDI3682#TechnicalResource"/>
        <rdfs:comment>One step of a process that transfers a status &quot;before&quot; (i.e., an input) to a status &quot;after&quot; (i.e., an output). 
Everything that has an input and an output may be a process operator (but could also be a process).
Everything that has an input and an output AND is contained within a process is a process operator.</rdfs:comment>
    </owl:Class>
    


    <!-- http://www.hsu-ifa.de/ontologies/VDI3682#Product -->

    <owl:Class rdf:about="http://www.hsu-ifa.de/ontologies/VDI3682#Product">
        <rdfs:subClassOf rdf:resource="http://www.hsu-ifa.de/ontologies/VDI3682#State"/>
        <rdfs:comment>A rather generic concepts to describe all sorts of raw, intermediate or final products. Can also be used to describe flow of materials.
[VDI 3682-1]</rdfs:comment>
    </owl:Class>
    


    <!-- http://www.hsu-ifa.de/ontologies/VDI3682#State -->

    <owl:Class rdf:about="http://www.hsu-ifa.de/ontologies/VDI3682#State">
        <owl:disjointWith rdf:resource="http://www.hsu-ifa.de/ontologies/VDI3682#SystemLimit"/>
        <owl:disjointWith rdf:resource="http://www.hsu-ifa.de/ontologies/VDI3682#TechnicalResource"/>
        <rdfs:comment>A State describes the actual state of a Product/Energy/Information. Exp.: status ante operationem and status post operationem.
[VDI3682-1]</rdfs:comment>
    </owl:Class>
    


    <!-- http://www.hsu-ifa.de/ontologies/VDI3682#SystemLimit -->

    <owl:Class rdf:about="http://www.hsu-ifa.de/ontologies/VDI3682#SystemLimit">
        <owl:disjointWith rdf:resource="http://www.hsu-ifa.de/ontologies/VDI3682#TechnicalResource"/>
        <rdfs:comment>The system limit determines the observation horizon of the process. In a broader sense, this can also be seen as the balance limit for incoming products/energy/information and outgoing products/energy/information.
[VDI 3682-1]</rdfs:comment>
    </owl:Class>
    


    <!-- http://www.hsu-ifa.de/ontologies/VDI3682#TechnicalResource -->

    <owl:Class rdf:about="http://www.hsu-ifa.de/ontologies/VDI3682#TechnicalResource">
        <rdfs:comment>The technical resource is able to implement certain processes and is an abstract description of a system.
[VDI 3682-1]</rdfs:comment>
    </owl:Class>
    


    <!-- http://www.w3.org/2002/07/owl#Thing -->

    <rdf:Description rdf:about="http://www.w3.org/2002/07/owl#Thing">
        <rdfs:comment>In order to check consistency, the following procedure is used:

First, the reasoner checks, whether the class expressions to hold for the ABox. If that is not the case, then a explanation of inconsistency can be accessed.

Second, SWRL rules are used to check the constency aspects that cannot be modelled through class expressions. These rules infer 4 &quot;Overall_X_Constent&quot; DataProperties. For the case that incremental rules were possible, other consistency attributes are inferred, so that in case of inconsistency a debugging can be started.

Explanation to class expressions in relation to DIN61360 definitions:

&quot;exactly&quot; is used for &quot;necessary&quot; (zwingend)
&quot;max&quot; is used for &quot;optinal&quot; (wahlfrei) with maximum restriction

If something is just &quot;optional&quot;, it will not occur in the class expression.

If a liability in DIN61360 states &quot;case dependend&quot; (bedingt), then this considered in a SWRL rule, which will give the DataProperties of &quot;x_Consistent&quot; to the Data_Element</rdfs:comment>
    </rdf:Description>
    


    <!-- 
    ///////////////////////////////////////////////////////////////////////////////////////
    //
    // General axioms
    //
    ///////////////////////////////////////////////////////////////////////////////////////
     -->

    <rdf:Description>
        <rdf:type rdf:resource="http://www.w3.org/2002/07/owl#AllDisjointClasses"/>
        <owl:members rdf:parseType="Collection">
            <rdf:Description rdf:about="http://www.hsu-ifa.de/ontologies/DINEN61360#Array"/>
            <rdf:Description rdf:about="http://www.hsu-ifa.de/ontologies/DINEN61360#Bag"/>
            <rdf:Description rdf:about="http://www.hsu-ifa.de/ontologies/DINEN61360#Boolean"/>
            <rdf:Description rdf:about="http://www.hsu-ifa.de/ontologies/DINEN61360#Integer"/>
            <rdf:Description rdf:about="http://www.hsu-ifa.de/ontologies/DINEN61360#List"/>
            <rdf:Description rdf:about="http://www.hsu-ifa.de/ontologies/DINEN61360#Real"/>
            <rdf:Description rdf:about="http://www.hsu-ifa.de/ontologies/DINEN61360#Set"/>
            <rdf:Description rdf:about="http://www.hsu-ifa.de/ontologies/DINEN61360#String"/>
        </owl:members>
    </rdf:Description>
</rdf:RDF>



<!-- Generated by the OWL API (version 4.5.9.2019-02-01T07:24:44Z) https://github.com/owlcs/owlapi -->

